Zcash/Snark.lean
@@ -44,6 +44,7 @@ import Zcash.Snark.Soundness.OperationLookups
 import Zcash.Snark.Soundness.OperationGates
 import Zcash.Snark.Soundness.OperationFixed
 import Zcash.Snark.Soundness.CircuitIntegration
+import Zcash.Snark.Soundness.TopLevelCircuit
 import Zcash.Snark.Soundness.PolynomialEnvironment
 import Zcash.Snark.Soundness.ActionAssignment
 import Zcash.Snark.Soundness.InnerProduct
